src/Ts_of_map_proof.thy
@@ -1,0 +1,394 @@
+(* [[file:~/workspace/agenda/myTasks.org::*proof%20ts_to_map_invariant][proof\ ts_to_map_invariant\ \[2/5\]:1]] *)
+theory Ts_of_map_proof
+imports Key_lt_order Find_tree_stack Insert_tree_stack (*Andrea_proof*)
+begin
+lemma set_butlast_lessThan:"set (butlast [0..<n]) = {0..<n -1}"
+apply (case_tac n,force+)
+done
+
+lemma map_addE1: "map_le f g --> (f++g = g)"
+apply (simp add:map_le_def)
+apply (simp add:map_add_def) 
+apply rule+
+ apply (case_tac " g x",force,force)
+done
+
+lemma map_addE2: "map_le f g --> (g++f = g)"
+apply (simp add:map_le_def)
+apply (simp add:map_add_def) 
+apply rule+
+apply (case_tac " f x",force,force)
+done
+
+lemma distinct_keys_in_leaf:
+"!  ms. total_order_key_lte --> wellformed_tree ms (Leaf(kvs)) --> distinct (map fst (List.concat (tree_to_leaves (Leaf(kvs)))))"
+apply simp
+apply rule+
+apply (erule exE)
+apply (subgoal_tac "keys_ordered (Leaf kvs)") prefer 2 apply (force simp add:wellformed_tree_def)
+apply (simp add:keys_ordered_def forall_subtrees_def rev_apply_def keys_ordered_1_def key_indexes_def set_butlast_lessThan Let_def atLeast0LessThan lessThan_def check_keys_def)
+apply (thin_tac "wellformed_tree ms (Leaf kvs)")
+apply (induct kvs,force)
+(*(a # kvs)*)
+apply simp
+apply (subgoal_tac "\<forall>i<length (kvs). key_lt (fst a) (fst (kvs ! i))") prefer 2
+ apply (subgoal_tac "\<forall>i<length (a#kvs) - 1. key_lt (fst ((a#kvs)!0)) (fst ((a#kvs) ! Suc i))")
+ prefer 2
+  apply rule+
+  apply (subgoal_tac "(a#kvs) ~= []") prefer 2 apply (force)
+  apply (subgoal_tac "!i : {0..<length (a#kvs) - Suc 0}. key_lt (fst ((a#kvs) ! i)) (fst ((a#kvs) ! Suc i))") prefer 2 apply force 
+  apply (smt One_nat_def Suc_mono atLeastLessThan_iff hd_smallest_in_list_sorted_by_key_lt length_Cons length_map length_tl less_Suc_eq list.sel(3) list.size(3) neq0_conv nth_map)
+ apply force
+apply (subgoal_tac "\<forall>i<length kvs - 1. key_lt (fst ((kvs) ! i)) (fst (kvs ! Suc i))")
+prefer 2
+ apply (metis Suc_diff_1 Suc_mono diff_0_eq_0 less_nat_zero_code neq0_conv nth_Cons_Suc)
+apply (thin_tac "\<forall>i<length kvs. key_lt (fst ((a # kvs) ! i)) (fst (kvs ! i))")
+apply rule
+ apply (metis imageE in_set_conv_nth key_lt_implies_neq)
+
+ apply (case_tac "kvs",force+)
+done
+
+lemma distinct_kv_in_tree:
+"!  ms. total_order_key_lte --> wellformed_tree ms t --> distinct (List.concat (tree_to_leaves t))"
+apply rule+
+apply (subgoal_tac "keys_consistent t") prefer 2 apply (force simp add:wellformed_tree_def)
+apply (subgoal_tac "! kvs. t = Leaf kvs --> distinct (map fst (List.concat (tree_to_leaves t)))") prefer 2 apply (metis distinct_keys_in_leaf)
+apply (thin_tac "wellformed_tree ms t")
+apply (induct t) prefer 2
+ apply (metis distinct_zipI1 zip_map_fst_snd)
+  
+ apply (case_tac x)
+ apply (rename_tac ks rs)
+ apply (simp add:snds_def sndsp.simps del:tree_to_leaves.simps)
+ apply (subgoal_tac "distinct (tree_to_leaves (Node (ks, rs)))")
+ prefer 2 
+  (* this goal should somehow use keys_consistent*)
+  apply (force intro:FIXME)
+ apply (subgoal_tac "! ys : set (tree_to_leaves (Node (ks, rs))). distinct ys")
+ prefer 2 
+  (*this goal should open the hp keys_consistent to allow the induction *)
+  apply (force intro:FIXME)
+ apply (subgoal_tac "!ys zs. ys \<in> set ((tree_to_leaves (Node (ks, rs)))) --> 
+                             zs \<in> set ((tree_to_leaves (Node (ks, rs)))) --> 
+                              ys \<noteq> zs --> set ys \<inter> set zs = {}")
+ prefer 2
+  (*this goal may be related to distinct (tree_to_leaves (Node (ks, rs)))*)
+  apply (force intro:FIXME)
+ apply (force simp add: distinct_concat)
+sorry
+
+lemma distinct_keys_in_leaves:
+"!  ms. total_order_key_lte --> wellformed_tree ms t --> distinct (map fst (List.concat (tree_to_leaves t)))"
+apply rule+
+apply (subgoal_tac "distinct (List.concat (tree_to_leaves t))") prefer 2 apply (simp add:distinct_kv_in_tree del:tree_to_leaves.simps)
+apply (unfold distinct_map inj_on_def id_def)
+apply rule+
+ apply force
+apply rule+
+ apply force
+apply clarsimp
+apply (subgoal_tac "(aa, b) = (aa,ba)") prefer 2
+ apply (subgoal_tac "x ~= xa --> (inter (set x) (set xa)) = {}") prefer 2 apply (fast intro:FIXME)
+ (*probably better to show directly that keys are unique?*)
+ apply (fast intro:FIXME)
+apply force
+done
+
+lemma map_le_subtrees:
+"! t ks rs ms. 
+let pt = (Node(ks,rs)) in
+(
+total_order_key_lte -->
+wellformed_tree ms pt -->
+t : set rs -->
+map_le (tree_to_map t) (tree_to_map pt))"
+apply (simp add:Let_def)
+apply rule+
+apply (erule exE)
+apply (subgoal_tac "distinct (map fst (List.concat (tree_to_leaves (Node(ks,rs)))))")
+prefer 2
+ apply (simp add:wellformed_context_1_def)
+ using distinct_keys_in_leaves apply force
+apply (subgoal_tac "? xs ys. rs = xs@t#ys")
+prefer 2
+ using split_list apply fast
+apply (erule exE)+
+apply (simp add:rev_apply_def map_le_def tree_to_map_def)
+apply rule+
+apply (rename_tac "key")
+apply (subgoal_tac "~ key : dom(map_of (concat (concat (map tree_to_leaves ys)))) & ~ key : dom(map_of (concat (concat (map tree_to_leaves xs))))")
+prefer 2
+ apply (simp add:dom_def map_of_eq_None_iff)
+ apply (simp add:keys_def rev_apply_def keys_1_def)
+ apply (erule conjE)+
+ apply (subgoal_tac "? xsks. fst ` (\<Union>x\<in>set xs. \<Union>x\<in>set (case x of Node (l, cs) \<Rightarrow> cs |> map tree_to_leaves |> concat | Leaf l \<Rightarrow> [l]). set x) = xsks") prefer 2 apply force
+ apply (erule exE)
+ apply simp
+ apply (subgoal_tac "? ysks. fst ` (\<Union>x\<in>set ys. \<Union>x\<in>set (case x of Node (l, cs) \<Rightarrow> cs |> map tree_to_leaves |> concat | Leaf l \<Rightarrow> [l]). set x) = ysks") prefer 2 apply force
+ apply (erule exE)
+ apply simp
+ apply (blast)
+apply (simp add:map_add_dom_app_simps(1) map_add_dom_app_simps(3))
+done
+
+lemma ctx_map_le: 
+"
+1 < length ctx -->
+wellformed_context ctx -->
+(
+let (_,((ks,rs),_),_) = hd ctx in
+let ctx' = tl ctx in
+map_le (tree_to_map (Node(ks,rs))) (ctx_to_map ctx'))
+"
+
+apply rule+
+apply (simp add:Let_def)
+apply (induct ctx,force)
+apply (rename_tac ctx_h ctx_t)
+apply simp
+apply (case_tac ctx_t,force)
+apply (rename_tac ctx_h1 ctx_t1)
+apply simp
+apply (subgoal_tac "? l ks rs i u. ctx_h = (l,((ks,rs),i),u)") prefer 2 apply force
+apply (erule exE)+
+apply simp
+apply (subgoal_tac "? l1 ks1 rs1 i1 u1. ctx_h1 = (l1,((ks1,rs1),i1),u1)") prefer 2 apply force
+apply (erule exE)+
+apply (subgoal_tac "ctx_to_map (ctx_h1 # ctx_t1) = (tree_to_map (Node(ks1,rs1)) ++ ctx_to_map ctx_t1)")
+prefer 2
+ apply (force intro:FIXME)
+apply simp
+apply (subgoal_tac "map_le (tree_to_map (Node (ks, rs))) (tree_to_map (Node (ks1, rs1)))")
+prefer 2
+ apply (force intro:FIXME)
+(*let's simplify the inductive hp*)
+apply (case_tac ctx_t1)
+ (*ctx_t1 = []*)
+ apply (force simp add:ctx_to_map_def)
+
+ (*ctx_t1 ~= []*)
+ apply (simp)
+ using map_addE1 map_le_trans apply fastforce
+done
+
+(*begin findmapts invariant*)
+definition invariant_find_map_fts :: "bool" where
+"invariant_find_map_fts = (
+!fts.
+let fts' = step_fts fts in
+let m_eq_m' = (
+ let m = fts_to_map fts in
+ (case fts' of None => True
+ | Some fts' =>
+ let m' = fts_to_map fts' in
+ m = m'))
+in
+total_order_key_lte -->
+wellformed_fts fts -->
+(case fts' of None => True | Some fts' => wellformed_fts fts') -->  (*FIXME: remove! this is given by Insert_step_up_proof*)
+m_eq_m')
+"
+(*end findmapts invariant*)
+
+lemma invariant_find_map_fts: "invariant_find_map_fts"
+apply (simp add:invariant_find_map_fts_def Let_def)
+apply rule+
+apply (case_tac "step_fts fts",force)
+apply simp
+apply (rename_tac fts')
+apply (simp add:step_fts_def)
+apply (subgoal_tac "? k t ctx. dest_f_tree_stack fts = (k,t,ctx)")
+prefer 2
+ apply (case_tac fts)
+ apply (rename_tac ts)
+ apply (case_tac ts)
+ apply (rename_tac f ctx)
+ apply (case_tac f)
+ apply (force simp add:dest_f_tree_stack_def)
+apply (erule exE)+
+apply simp
+apply (subgoal_tac "? lb rb. ((case ctx of [] \<Rightarrow> (None, None) | (lb, xb, xc) # xa => (lb, xc)) = (lb,rb))") prefer 2 apply force
+apply (erule exE)+
+apply simp
+apply (case_tac "t") prefer 2 apply force
+apply simp
+apply (rename_tac ksrs)
+apply (case_tac ksrs)
+apply (rename_tac ks rs)
+apply (simp add:Let_def)
+apply (subgoal_tac "? l u. get_lower_upper_keys_for_node_t ks lb (search_key_to_index ks k) rb = (l,u)") prefer 2 apply force
+apply (erule exE)+
+apply simp
+apply (thin_tac "ksrs=_")
+apply (thin_tac "t=_")
+apply (simp add:fts_to_map_def)
+apply (subgoal_tac "? t' ctx'. dest_f_tree_stack fts' = (k,t',ctx')")
+prefer 2
+ apply (case_tac fts)
+ apply (rename_tac ts)
+ apply (case_tac ts)
+ apply (rename_tac f ctx)
+ apply (case_tac f)
+ apply (force simp add:dest_f_tree_stack_def)
+apply (erule exE)+
+apply (simp add:rev_apply_def)
+apply (subgoal_tac "? m_kvs. tree_to_map t' = m_kvs") prefer 2 apply force
+apply (erule exE)
+apply (subgoal_tac "? ctx'_h.  (l,((ks,rs),(search_key_to_index ks k)),u) = ctx'_h") prefer 2 apply force
+apply (erule exE)
+apply (subgoal_tac "ctx' =ctx'_h#ctx")
+prefer 2
+ apply (drule_tac t="ctx'_h" in sym)
+ apply (drule_tac t="fts'" in sym)
+ apply (force simp add:dest_f_tree_stack_def)
+apply (subgoal_tac "? map_of_ctx. (ctx_to_map ctx) = map_of_ctx") prefer 2 apply force
+apply (erule exE)
+apply simp
+apply (subgoal_tac "? map_of_ctx'_h. tree_to_map (Node(ks,rs)) = map_of_ctx'_h") prefer 2 apply force
+apply (erule exE)
+apply simp
+apply (subgoal_tac "ctx ~= [] --> ctx_to_map ctx' = map_of_ctx'_h++(map_of_ctx)")
+prefer 2
+ apply (case_tac ctx) apply force
+ apply simp
+ apply (rename_tac ctx_h ctx_t)
+ apply (subgoal_tac "map_le map_of_ctx'_h map_of_ctx")
+ prefer 2
+  apply (subgoal_tac "wellformed_context ctx'") prefer 2 apply (force simp add:wellformed_fts_def)
+  apply (subgoal_tac "1 < length ctx'") prefer 2 apply force
+  using ctx_map_le apply (fastforce)
+ apply (subgoal_tac "ctx_to_map ctx' = map_of_ctx ++ map_of_ctx'_h") prefer 2 apply (force simp add: tree_to_map_def ctx_to_map_def)
+ apply (metis map_le_iff_map_add_commute map_le_map_add map_le_trans)
+apply (simp add:rev_apply_def)
+apply (subgoal_tac "m_kvs ++ map_of_ctx'_h = map_of_ctx'_h")
+prefer 2
+ apply (subgoal_tac "map_le m_kvs map_of_ctx'_h")
+ prefer 2
+  (*this demonstration should be equivalent to the other subgoal about map_le*)
+  (*wellformed_fts_1 tells us that t' belongs to the context*)
+  (*probably worth creating a fake ctx head to reuse the ctx_map_le lemma, nope because we would not know this fake is wf_ctx *)
+  (*we need a predicate that is more general, something like:
+    ! t. wf_tree t --> ! subtree. map_le msubtree mt
+  can I reuse this for ctx? I think so, since all I have to do is showing that ctx heads are subnodes.
+  *)
+  apply (subgoal_tac "? ms. (if ctx = [] then Some Small_root_node_or_leaf else None) = ms") prefer 2 apply force
+  apply (erule exE)+
+  apply (subgoal_tac "t' : set rs & wellformed_tree ms (Node(ks,rs))")
+  prefer 2
+   apply (simp add:wellformed_fts_def)
+   apply (simp add:wellformed_fts_focus_def)
+   apply (simp add:wellformed_fts_1_def)
+   apply (drule_tac t=ctx'_h in sym)
+   apply simp
+   apply (subgoal_tac "search_key_to_index ks k < length rs")
+   prefer 2
+    apply (simp add:search_key_to_index_def)
+    apply (subgoal_tac "length ks = (length rs -1) & length rs ~= 0")
+    prefer 2 
+     (*wf_tree Node(ks,rs)*)
+     apply (force intro:FIXME)
+    apply (simp add:Let_def)
+    apply (case_tac "find (\<lambda>x. key_lt k (ks ! x)) [0..<length rs - Suc 0]",force)
+    apply simp
+    apply (simp add:find_Some_iff)
+    apply (erule exE)+
+    apply force
+   apply force
+  using map_le_subtrees
+  apply (drule_tac x="t'" in spec)
+  apply (drule_tac x="ks" in spec)
+  apply (drule_tac x="rs" in spec)
+  apply (drule_tac x="ms" in spec)
+  apply force
+ apply (force simp add: map_addE1)
+apply (case_tac "ctx")
+apply (force simp add:tree_to_map_def ctx_to_map_def rev_apply_def)+
+done
+
+
+(*begin stepupmapts invariant*)
+definition invariant_step_up_map_its :: "bool" where
+"invariant_step_up_map_its = (
+!its.
+let its' = step_up its in
+let m_eq_m' = (
+ let m = its_to_map its in
+ (case its' of None => True
+ | Some its' =>
+ let m' = its_to_map its' in
+ m = m'))
+in
+total_order_key_lte -->
+wellformed_ts its -->
+(case its' of None => True | Some its' => wellformed_ts its') -->  (*FIXME: remove! this is given by Insert_step_up_proof*)
+m_eq_m')
+"
+(*end stepupmapts invariant*)
+
+lemma invariant_step_up_map_its: "invariant_step_up_map_its"
+apply (simp add:invariant_step_up_map_its_def Let_def)
+apply rule+
+apply (case_tac "step_up its",force)
+apply simp
+apply (rename_tac ts)
+apply (simp add:step_up_def)
+apply (subgoal_tac "? f ctx. its = Tree_stack (Focus f, ctx)")
+prefer 2
+ apply (case_tac its)
+ apply (rename_tac fctx)
+ apply (case_tac fctx)
+ apply (rename_tac tf ctx)
+ apply (case_tac tf,force)
+apply (erule exE)+
+apply (simp add:dest_ts_def)
+apply (case_tac ctx,force)
+apply (rename_tac ctx_h ctx_t)
+apply simp
+apply (subgoal_tac "? l ks rs i u. ctx_h = (l,((ks,rs),i),u)") prefer 2 apply force
+apply (erule exE)+
+apply simp
+apply (drule_tac t = ts in sym)
+apply (subgoal_tac "? f' . (update_focus_at_position (ks, rs) i f) = f' ") prefer 2 apply (force)
+apply (erule exE)
+apply (simp add:its_to_map_def dest_ts_def)
+apply (subgoal_tac "(ctx_to_map ((l, ((ks, rs), i), u) # Nil)  ++ its_f_to_map f) = (its_f_to_map f')")
+(*FIXME move demonstration @ here*)
+apply (case_tac "ctx_t = []")
+ (*ctx_t = []*)
+ apply (subgoal_tac "ctx_to_map [] = empty") prefer 2 apply (force simp add:ctx_to_map_def)
+ apply force
+
+ (*ctx_t ~= []*)
+ apply (simp add:ctx_to_map_def)
+ apply (metis map_add_assoc)
+(*FIXME demonstration @ begin*)
+(*I want to show that the f' subtrees are composed by rs1++x@rs2 where x is f*)
+
+apply (simp add:ctx_to_map_def) (*I want to say that f' is composed by rs1@f++rs2*)
+apply (force intro:FIXME)
+done
+
+(*begin stepbottommapts invariant*)
+definition invariant_step_bottom_map_its :: "bool" where
+"invariant_step_bottom_map_its = (
+!fts k v.
+let its = step_bottom fts v in
+let m_eq_m' = (
+ let m = fts_to_map fts in
+ (case its of None => True
+ | Some its =>
+ let m' = its_to_map its in
+ m' = m(k \<mapsto> v)))
+in
+total_order_key_lte -->
+wellformed_fts fts -->
+(case its of None => True | Some its => wellformed_ts its) -->  (*FIXME: remove! this is given by Insert_step_bottom_proof*)
+m_eq_m')
+"
+(*end stepbottommapts invariant*)
+
+lemma invariant_step_bottom_map_its: "invariant_step_bottom_map_its"
+sorry
+end
+(* proof\ ts_to_map_invariant\ \[2/5\]:1 ends here *)
